add new dropWhile constant to listTheory, and various lemmas

src/list/src/listSimps.sml
@@ -351,7 +351,7 @@ val list_rws = computeLib.add_thms
       NULL_DEF, CONS_11, NOT_CONS_NIL, NOT_NIL_CONS, MEM, EXISTS_DEF, EVERY_DEF,
       ZIP, UNZIP, TAKE_compute, DROP_compute, PAD_LEFT, PAD_RIGHT, isPREFIX,
       REVERSE_REV, REV_DEF, SUM_SUM_ACC, SUM_ACC_DEF,
-      FILTER, FOLDL, FOLDR,
+      FILTER, FOLDL, FOLDR, dropWhile_DEF,
       EL_restricted, EL_simp_restricted, SNOC,
       computeLib.lazyfy_thm list_case_compute,
       list_size_def, ALL_DISTINCT, FRONT_DEF, LAST_compute,
